compcert/Events2.v is a patch of compcert/Events.v that slightly modifies mem_unchanged_on (used in the semantics of external calls) to make it transitively closed over unmapped and out of reach addresses.  A couple of these transitivity proofs are included in the new file.
The new definition of "compilable" extension and proof of extension simulation 
(coming soon, hopefully) will make extensive use of these transitivity
lemmas.
 
NOTE: Events2.v builds in the CompCert trunk as a replacement for Events.v, 
after a couple small modifications to backend/Stackingproof.v.  If the 
transitivity lemmas really do prove useful, it may make sense to attempt 
to merge the new file into the CompCert distribution.

veric/extension.v
@@ -2,6 +2,7 @@ Load loadpath.
 Require Import msl.predicates_hered.
 Require Import veric.sim veric.step_lemmas veric.base veric.expr veric.extspec 
                veric.juicy_extspec.
+Require Import compcert.Events2.
 Require Import ListSet.
 
 Set Implicit Arguments.
@@ -138,13 +139,13 @@ Module Extension. Section Extension.
   (handled: list AST.external_function). (** functions handled by this extension *)
 
  Record Sig := Make {
- (** generalized projection of core [i] from state [s] *)
+ (** Generalized projection of core [i] from state [s] *)
    proj_core : forall i:nat, xT -> option (cT i);
    core_exists : forall ge i s c' m s' m', 
      corestep esem ge s m s' m' -> proj_core i s' = Some c' -> 
      exists c, proj_core i s = Some c;
    
- (** the active (i.e., currently scheduled) core *)
+ (** The active (i.e., currently scheduled) core *)
    active : xT -> nat;
    active_csem : forall s, exists CS, csem (active s) = Some CS;
    active_proj_core : forall s, exists c, proj_core (active s) s = Some c;
@@ -410,3 +411,198 @@ Record Sig := Make {extension_sound: safety_interpolant E -> safe_extension E}.
 
 End EXTENSION_SOUNDNESS. End EXTENSION_SOUNDNESS.
 
+(* Here we begin to develop a notion of compilable extension *)
+
+Lemma mem_unchanged_on_trans: 
+  forall P m m'' m',
+  mem_unchanged_on P m m'' -> 
+  mem_unchanged_on P m'' m' -> 
+  mem_unchanged_on P m m'.
+Proof.
+intros until m'; intros [H1 H2] [H3 H4].
+split.
+intros b ofs k p H5 H6 H7.
+specialize (H1 _ _ _ _ H5 H6 H7).
+eapply H3; eauto.
+eapply Mem.perm_valid_block; eauto.
+intros until v; intros H5 H6 H7.
+specialize (H2 _ _ _ _ H5 H6 H7).
+eapply H4; eauto.
+apply Mem.load_valid_access in H2.
+apply Mem.valid_access_implies with (p2 := Nonempty) in H2.
+eapply Mem.valid_access_valid_block; eauto.
+econstructor; eauto.
+Qed.
+
+Lemma mem_unchanged_on_weaken:
+  forall (P P': block -> Z -> Prop) m m',
+  (forall b ofs, P' b ofs -> P b ofs) -> 
+  mem_unchanged_on P m m' -> 
+  mem_unchanged_on P' m m'.
+Proof.
+intros until m'; intros H1 [H2 H3].
+split.
+intros until p; intros H4 H5 H6.
+solve[apply (H2 _ _ _ _ H4 (H1 _ _ H5) H6)].
+intros until v; intros H4 H5 H6.
+eapply H3; eauto.
+Qed.
+
+(*This is an [F,V]-independent definition of meminj_preserves_globals*)
+Definition meminj_preserves_globals (globals: list block) f :=
+  (forall b, In b globals -> f b = Some (b, 0)) /\
+  (forall b1 b2 delta, In b2 globals -> f b1 = Some (b2, delta) -> b1=b2).
+
+Lemma meminj_preserves_globals_incr: 
+  forall globals f f' m1 m2,
+  inject_incr f f' -> 
+  inject_separated f f' m1 m2 -> 
+  Mem.inject f m1 m2 -> 
+  meminj_preserves_globals globals f -> 
+  meminj_preserves_globals globals f'.
+Proof.
+intros until m2; intros H1 SEP INJ [H2 H3].
+split.
+intros b H4.
+specialize (H2 _ H4).
+solve[eapply H1; eauto].
+intros until delta; intros H4 H5.
+specialize (H3 b1 b2 delta H4).
+case_eq (f b1).
+intros [b' ofs'] H6.
+specialize (H1 _ _ _ H6).
+rewrite H1 in H5; inv H5.
+apply H3; auto.
+intros H6.
+unfold inject_separated in SEP.
+destruct (SEP _ _ _ H6 H5) as [H7 H8].
+specialize (H2 _ H4).
+elimtype False.
+apply H8.
+apply (Mem.valid_block_inject_2 _ m1 _ _ _ _ H2); auto.
+Qed.
+
+Module CompilableSem. Section CompilableSem.
+ Variables (F V: Type).
+ Variable (sem: list block -> mem -> mem -> Prop).
+
+ Inductive Sig: Type := Make: forall 
+   (PERM: forall ge m1 m1' b ofs p,
+     sem ge m1 m1' ->      
+     Mem.valid_block m1 b -> 
+     Mem.perm m1' b ofs Max p -> Mem.perm m1 b ofs Max p)
+   (VALID: forall ge m1 m1' b, 
+     sem ge m1 m1' -> 
+     Mem.valid_block m1 b -> Mem.valid_block m1' b)
+   (EXTENSIBLE: forall ge m1 m1' f m2,
+     meminj_preserves_globals ge f ->
+     sem ge m1 m1' -> 
+     Mem.extends m1 m2 ->
+     exists m2',
+       sem ge m2 m2' /\
+       Mem.extends m1' m2' /\
+       mem_unchanged_on (loc_out_of_bounds m1) m2 m2')
+   (INJECTIBLE: forall ge m1 m1' f m2,
+     meminj_preserves_globals ge f ->
+     sem ge m1 m1' -> 
+     Mem.inject f m1 m2 ->
+     exists f', exists m2',
+       sem ge m2 m2' /\
+       Mem.inject f' m1' m2' /\
+       mem_unchanged_on (loc_unmapped f) m1 m1' /\
+       mem_unchanged_on (loc_out_of_reach f m1) m2 m2' /\
+       inject_incr f f' /\
+       inject_separated f f' m1 m2),
+   (*other conditions might be required here*)
+   Sig.
+
+End CompilableSem.
+
+Section CompilableTrans.
+Variables (sem1 sem2: list block -> mem -> mem -> Prop).
+
+Definition sem12 ge m1 m3 := exists m2, sem1 ge m1 m2 /\ sem2 ge m2 m3.
+
+Lemma compilable_trans: Sig sem1 -> Sig sem2 -> Sig sem12.
+Proof.
+intros H1 H2;
+destruct H1 as [PERM1 VALID1 EXT1 INJ1]; 
+destruct H2 as [PERM2 VALID2 EXT2 INJ2].
+constructor.
+(*PERM*)
+clear -VALID1 VALID2 PERM1 PERM2.
+intros until p; intros H1 H2.
+destruct H1 as [m1'' [SEM1 SEM2]]; eauto.
+(*VALID*)
+clear -VALID1 VALID2 PERM1 PERM2.
+intros until b; intros H1 H2.
+destruct H1 as [m1'' [SEM1 SEM2]]; eauto.
+(*EXTENSIBLE*)
+intros until m2; intros H1 H2 H3.
+destruct H2 as [m1'' [SEM1 SEM2]].
+exploit EXT1; eauto; intros [m2'' [H4 [H5 H6]]].
+exploit EXT2; eauto; intros [m2' [H7 [H8 H9]]].
+exists m2'; split. 
+exists m2''; split; auto.
+split; auto.
+generalize (@mem_unchanged_outofbounds_trans _ _ _ _ m2' 
+ H3 H5 H6); intro H10.
+spec H10; eauto.
+(*INJECTIBLE*)
+intros until m2; intros H1 H2 H3.
+destruct H2 as [m1'' [SEM1 SEM2]].
+exploit INJ1; eauto; intros [f'' [m2'' [H4 [H5 [H6 [H7 [H8 H9]]]]]]].
+exploit (INJ2 ge m1'' m1' f''); eauto.
+assert (GLOB_INCR: meminj_preserves_globals ge f'').
+ solve[eapply meminj_preserves_globals_incr; eauto].
+eapply GLOB_INCR; eauto.
+intros [f' [m2' [H10 [H11 [H12 [H13 [H14 H15]]]]]]].
+assert (MEMINJ_COMP: 
+ forall f f' m1 m2 m3,
+   Mem.inject f m1 m2 -> Mem.inject f' m2 m3 -> 
+   Mem.inject (compose_meminj f f') m1 m3).
+ solve[intros; eapply Mem.inject_compose; eauto].
+assert (TRANS: forall P m m'' m',
+  mem_unchanged_on P m m'' -> 
+  mem_unchanged_on P m'' m' -> 
+  mem_unchanged_on P m m').
+ intros; eapply mem_unchanged_on_trans; eauto.
+assert (WEAKEN: forall (P P': block -> Z -> Prop) m m',
+  (forall b ofs, P' b ofs -> P b ofs) -> 
+  mem_unchanged_on P m m' -> 
+  mem_unchanged_on P' m m').
+ intros; eapply mem_unchanged_on_weaken; eauto.
+exists f'; exists m2'; split.
+exists m2''; split; auto.
+split; auto.
+split; auto.
+eapply mem_unchanged_unmapped_trans; eauto.
+split; auto.
+apply mem_unchanged_outofreach_trans
+ with (m2 := m1'') (m2' := m2'') (f2 := f''); auto.
+intros; eapply VALID1; eauto.
+intros.
+eapply PERM1; eauto.
+split; auto.
+eapply inject_incr_trans; eauto.
+clear - SEM1 SEM2 H4 H10 H8 H9 H14 H15 VALID1 VALID2.
+unfold inject_separated in H9, H15|-*.
+intros until delta; intros H1 H2.
+case_eq (f'' b1).
+intros [b1' ofs1'] H3.
+rewrite (H14 _ _ _ H3) in H2.
+inv H2.
+eapply H9; eauto.
+intros H3.
+specialize (H15 _ _ _ H3 H2).
+destruct H15.
+split; intro.
+apply H.
+eapply VALID1; eauto.
+apply H0.
+eapply VALID1; eauto.
+Qed.
+
+End CompilableTrans.
+
+End CompilableSem.
